src/StandardLibrary/Orders.dfy
@@ -1,0 +1,151 @@
+include "UInt.dfy"
+  
+module {:extern "STLOrders"} StandardLibrary.Orders {
+  export
+    reveals Reflexive, AntiSymmetric, Transitive, Connected, TotalOrdering, Trichotomous
+    reveals LexicographicByteSeqBelow, LexicographicByteSeqBelowAux
+    provides AboutLexicographicByteSeqBelow
+    provides UInt
+    
+  import opened UInt
+
+  /*
+   * Properties of relations
+   *
+   */
+  
+  predicate Reflexive<T(!new)>(R: (T, T) -> bool) {
+    forall x :: R(x, x)
+  }
+  
+  predicate AntiSymmetric<T(!new)>(R: (T, T) -> bool) {
+    forall x, y :: R(x, y) && R(y, x) ==> x == y
+  }
+
+  predicate Transitive<T(!new)>(R: (T, T) -> bool) {
+    forall x, y, z :: R(x, y) && R(y, z) ==> R(x, z)
+  }
+
+  predicate Connected<T(!new)>(R: (T, T) -> bool) {
+    forall x, y :: R(x, y) || R(y, x)
+  }
+
+  predicate TotalOrdering<T(!new)>(R: (T, T) -> bool) {
+    && Reflexive(R)
+    && AntiSymmetric(R)
+    && Transitive(R)
+    && Connected(R)
+  }
+
+  /*
+   * For an ordering "R" to be _trichotomous_ means that for any two "x" and "y",
+   * EXACTLY one of the following three conditions holds:
+   *   - R(x, y)
+   *   - x == y
+   *   - R(y, x)
+   * Note that being trichotomous implies being irreflexive.
+   */
+  predicate Trichotomous<T(!new)>(R: (T, T) -> bool) {
+    (forall x, y :: R(x, y) || x == y || R(y, x)) &&  // at least one of the three
+    (forall x, y :: R(x, y) && R(y, x) ==> false) &&  // not both of the R's
+    (forall x, y :: R(x, y) ==> x != y)  // not an R and the equality
+  }
+
+  /*
+   * Useful orderings
+   *
+   * In what follows, the identifier "less" is used to denote a relation
+   * that is irreflexive, like "<" on numbers. The identifier "below" is used
+   * to denote a relation that is reflexive, like "<=" on numbers.
+   */
+
+  /*
+   * Here is an example relation and a lemma that says the relation is appropriate for use in
+   * lexicographic orderings.
+   */
+
+  lemma UInt8LessIsTrichotomousTransitive()
+    ensures Trichotomous(UInt8Less)
+    ensures Transitive(UInt8Less)
+  {
+  }
+
+  /*
+   * Reflexive lexicographical comparison of byte sequences
+   */
+  
+  predicate method LexicographicByteSeqBelow(x: seq<uint8>, y: seq<uint8>) {
+    LexicographicByteSeqBelowAux(x, y, 0)
+  }
+  
+  predicate method LexicographicByteSeqBelowAux(x: seq<uint8>, y: seq<uint8>, n: nat)
+    requires n <= |x| && n <= |y|
+    decreases |x| - n
+  {
+    || n == |x|
+    || (n != |y| && x[n] < y[n])
+    || (n != |y| && x[n] == y[n] && LexicographicByteSeqBelowAux(x, y, n + 1))
+  }
+
+  lemma AboutLexicographicByteSeqBelow()
+    ensures TotalOrdering(LexicographicByteSeqBelow)
+  {
+    assert Reflexive(LexicographicByteSeqBelow) by {
+      forall x, n | 0 <= n <= |x| {
+        AboutLexicographicByteSeqBelowAux_Reflexive(x, n);
+      }      
+    }
+    assert AntiSymmetric(LexicographicByteSeqBelow) by {
+      forall x, y, n: nat |
+        n <= |x| && n <= |y| && x[..n] == y[..n] &&
+        LexicographicByteSeqBelowAux(x, y, n) && LexicographicByteSeqBelowAux(y, x, n)
+      {
+        AboutLexicographicByteSeqBelowAux_AntiSymmetric(x, y, n);
+      }
+    }
+    assert Transitive(LexicographicByteSeqBelow) by {
+      forall x, y, z, n: nat |
+        n <= |x| && n <= |y| && n <= |z| &&
+        LexicographicByteSeqBelowAux(x, y, n) && LexicographicByteSeqBelowAux(y, z, n)
+      {
+        AboutLexicographicByteSeqBelowAux_Transitive(x, y, z, n);
+      }
+    }
+    assert Connected(LexicographicByteSeqBelow) by {
+      forall x, y, n: nat | n <= |x| && n <= |y| {
+        AboutLexicographicByteSeqBelowAux_Connected(x, y, n);
+      }
+    }
+  }
+  
+  lemma AboutLexicographicByteSeqBelowAux_Reflexive(x: seq<uint8>, n: nat)
+    requires n <= |x|
+    ensures LexicographicByteSeqBelowAux(x, x, n)
+    decreases |x| - n
+  {
+  }
+
+  lemma AboutLexicographicByteSeqBelowAux_AntiSymmetric(x: seq<uint8>, y: seq<uint8>, n: nat)
+    requires n <= |x| && n <= |y|
+    requires x[..n] == y[..n]
+    requires LexicographicByteSeqBelowAux(x, y, n) && LexicographicByteSeqBelowAux(y, x, n)
+    ensures x == y
+    decreases |x| - n
+  {
+  }
+
+  lemma AboutLexicographicByteSeqBelowAux_Transitive(x: seq<uint8>, y: seq<uint8>, z: seq<uint8>, n: nat)
+    requires n <= |x| && n <= |y| && n <= |z|
+    requires LexicographicByteSeqBelowAux(x, y, n) && LexicographicByteSeqBelowAux(y, z, n)
+    ensures LexicographicByteSeqBelowAux(x, z, n)
+    decreases |x| - n
+  {
+  }
+
+  lemma AboutLexicographicByteSeqBelowAux_Connected(x: seq<uint8>, y: seq<uint8>, n: nat)
+    requires n <= |x| && n <= |y|
+    ensures LexicographicByteSeqBelowAux(x, y, n) || LexicographicByteSeqBelowAux(y, x, n)
+    decreases |x| - n
+  {
+  }
+}
