src/StandardLibrary/Sorting.dfy
@@ -1,0 +1,42 @@
+include "Orders.dfy"
+  
+module {:extern "STLSorting"} StandardLibrary.Sorting {
+  export
+    provides SelectionSort
+    provides Orders
+
+  import Orders
+    
+  /*
+   * Selection sort
+   */
+  
+  method SelectionSort<Data>(a: array<Data>, below: (Data, Data) -> bool)
+    requires Orders.Transitive(below) && Orders.Connected(below)
+    modifies a
+    ensures multiset(a[..]) == old(multiset(a[..]))
+    ensures forall i, j :: 0 <= i < j < a.Length ==> below(a[i], a[j])
+  {
+    var m := 0;
+    while m < a.Length
+      invariant 0 <= m <= a.Length
+      invariant multiset(a[..]) == old(multiset(a[..]))
+      invariant forall i, j :: 0 <= i < j < m ==> below(a[i], a[j])
+      invariant forall i, j :: 0 <= i < m <= j < a.Length ==> below(a[i], a[j])
+    {
+      // pick mindex to be the index of the smallest element in a[m..]
+      var mindex, n := m, m + 1;
+      while n < a.Length
+        invariant m <= mindex < n <= a.Length
+        invariant forall i :: m <= i < n ==> below(a[mindex], a[i])
+      {
+        if !below(a[mindex], a[n]) {
+          mindex := n;
+        }
+        n := n + 1;
+      }
+      a[m], a[mindex] := a[mindex], a[m];
+      m := m + 1;
+    }
+  }
+}
